theories/zoo_saturn/bqueue_spsc__types.v
@@ -5,22 +5,22 @@ Require Export zoo_std.array.
 Require Import zoo.options.
 
 Notation "'data'" := (
-  in_type "zoo_saturn.spsc_bqueue.t" 0
+  in_type "zoo_saturn.bqueue_spsc.t" 0
 )(in custom zoo_field
 ).
 Notation "'front'" := (
-  in_type "zoo_saturn.spsc_bqueue.t" 1
+  in_type "zoo_saturn.bqueue_spsc.t" 1
 )(in custom zoo_field
 ).
 Notation "'front_cache'" := (
-  in_type "zoo_saturn.spsc_bqueue.t" 2
+  in_type "zoo_saturn.bqueue_spsc.t" 2
 )(in custom zoo_field
 ).
 Notation "'back'" := (
-  in_type "zoo_saturn.spsc_bqueue.t" 3
+  in_type "zoo_saturn.bqueue_spsc.t" 3
 )(in custom zoo_field
 ).
 Notation "'back_cache'" := (
-  in_type "zoo_saturn.spsc_bqueue.t" 4
+  in_type "zoo_saturn.bqueue_spsc.t" 4
 )(in custom zoo_field
 ).
